\documentclass{article}
\usepackage[utf8]{inputenc}
\usepackage{amsmath}
\usepackage{mathtools}
\usepackage{amsthm}
\usepackage{graphicx}
\usepackage{tabularx}
\usepackage{mathtools}
\usepackage{mathrsfs}
\usepackage{enumerate}
\usepackage{amssymb}
\usepackage{accents}
\usepackage{commath}
\usepackage{yfonts}
\usepackage{float}
\usepackage{array}
\usepackage{tikz-cd}
\usepackage{listings}

\title{Stat3004 Assignment 3}
\author{Dominic Scocchera}
\date{April 2023}

\newtheorem{theorem}{Theorem}
\newtheorem{corollary}{Corollary}
\newtheorem{lemma}[theorem]{Lemma}

\begin{document}
\maketitle
%https://math.stackexchange.com/questions/2172959/joint-mass-function-of-a-poisson-process
\section*{Q1}
First we note that $N((a,b])\sim Poi(2\cdot(b-a))$.
\subsection*{a)}
\begin{align*}
\mathbb{P}(N_{t_1}=n_1,N_{t_2}=n_2)&=\mathbb{P}(N_{2}=7,N_{12}=10)\\
&=\mathbb{P}(N_2=7,N_{12-2}=10-7)\\
&=\mathbb{P}(N_2=7)\mathbb{P}(N_{10}=3)\\
&=e^{-2\cdot2}\frac{(2\cdot2)^7}{7!}e^{-2\cdot10}\frac{(2\cdot10)^{3}}{3!}\\
&\approx1.636291121\times10^{-7}\\
\end{align*}
\subsection*{b)}
\begin{align*}
\mathbb{P}(N(1, t_1]=n_1, N(t_1-1,t_2]=n_2)&=\mathbb{P}(N(1,2]=7, N(1,12]=10)\\
&=\mathbb{P}(N(1,2]=7, N(2,12]=3)\\
&=\mathbb{P}(N(1,2]=7)\mathbb{P}(N(2,12]=3)\\
&=\frac{e^{-2}(2)^7}{7!}\frac{e^{-20}(20)^3}{3!}\\
&\approx 9.4458178806\times10^{-9}\\
\end{align*}
\subsection*{c)}
\begin{align*}
\mathbb{E}[N(1,t_1]\;|\;N(t_1-1,t_2]=n_2]&=\mathbb{E}[N(1,2]\;|\;N(1,12]=10]\\
&=\sum_{t\geq0}t\cdot\mathbb{P}(N(1,2]=t|N(1,12]=10)\\
&=\sum_{t=0}^{10}t\cdot\frac{\mathbb{P}(N(1,2]=t,N(1,12]=10)}{\mathbb{P}(N(1,12]=10)}\\
&=\frac{1}{\mathbb{P}(N(1,12]=10)}\sum_{t=0}^{10}t\cdot\mathbb{P}(N(1,2]=t,N(2,12]=10-t)\\
&=\frac{1}{\mathbb{P}(N(1,12]=10)}\sum_{t=0}^{10}t\cdot\mathbb{P}(N(1,2]=t)\mathbb{P}(N(2,12]=10-t)\\
&=\frac{1}{\frac{e^{-22}(22)^{10}}{10!}}\sum_{t=0}^{10}t\cdot\frac{e^{-2}(2)^t}{t!}\frac{e^{-20}(20)^{10-t}}{(10-t)!}\\
&=\frac{10}{11}\\
\end{align*}
\subsection*{d)}
\begin{align*}
\mathbb{E}[N(t_1-1,t_2]\;|\;N(1,t_1]=n_1]&=\mathbb{E}[N(1,12]\;|\;N(1,2]=7]\\
&=\sum_{t\geq0}t\cdot\mathbb{P}(N(1,12]=t|N(1,2]=7)\\
&=\sum_{t\geq0}t\cdot\mathbb{P}(N(1,12]=t|N(1,2]=7)\\
&=\sum_{t\geq0}t\cdot\frac{\mathbb{P}(N(1,12]=t,N(1,2]=7)}{\mathbb{P}(N(1,2]=7)}\\
&=\sum_{t\geq0}t\cdot\frac{\mathbb{P}(N(2,12]=t+7,N(1,2]=t)}{\mathbb{P}(N(1,2]=7)}\\
\end{align*}
\section*{Q2}
\section*{Q3}
\subsection*{a)}
\subsection*{b)}
\subsection*{c)}
\section*{Q4}
\subsection*{a)}
\subsection*{b)}
\subsection*{c)}
\subsection*{d)}
\end{document}